\documentclass[14pt]{article}

\usepackage{repsty}


\begin{document}

The original expression for the standard error:	
\begin{equation}
\begin{cases}
		\SE{\hat{\omega}}^2 &= \frac{\SD{\obs}^2}{\Nozc\cdot g(\Nzc)\cdot \sum_{s=1}^{\Nzc}\sum_{j=1}^{\Nozc} w_{js} (t_{js} - \avg{t}_w)^2}, \\
		g(\Nzc) &= \frac{1-\exp{(-\sfrac{\pi}{\omega\tau_d}\cdot \Nzc)}}{1 - \exp{(-\sfrac{\pi}{\omega\tau_d})}}.
\end{cases}
\end{equation}
	
If our sample consists of observations made exclusively at the signal nodes with error standard deviation $\SD{\obs}$: $\Nozc = 1$, $w_{js} = w_{1s} = 1/\Nzc$,\footnote{This is actually false; a succeeding node observation carries exponentially less information than a preceding one because of decoherence, hence $w_{1s} = w_{11}\exp\bkt{-\frac{\pi}{\omega\tau_d}(s-1)}$.} and
\begin{equation}
	\begin{cases}
	\SE{\hat{\omega}}^2 &= \frac{\Nzc}{g(\Nzc)}\cdot \frac{\SD{\obs}^2}{\sum_{s=1}^{\Nzc}(t_{1s} - \avg{t}_w)^2}, \\
	t_{1s} &= h\cdot s, ~ h = \frac{1}{2}\frac{1}{2\pi\omega}.
	\end{cases}
\end{equation}

\begin{align*}
	\avg{t}_w &= \Nzc^{-1}\sum_{s=1}^{\Nzc}h\cdot s = \frac{h}{2}(\Nzc+1), \\
	\sum_{s=1}^{\Nzc}(t_{1s} - \avg{t}_w)^2 &= \sum_s t_{1s}^2 - \Nzc\avg{t}_w^2 \\
			&= h^2\frac{\Nzc(\Nzc+1)(2\Nzc+1)}{6} - h^2\frac{\Nzc(\Nzc+1)^2}{4} \\
			&= \frac{h^2}{12}\Nzc(\Nzc^2-1).
\end{align*}
	
\begin{align}
	\SE{\hat{\omega}}^2 &= \frac{12}{g(\Nzc)}\frac{\SD{\obs}^2}{h^2(\Nzc^2-1)} \approx \frac{12}{g(\Nzc)}\frac{\SD{\obs}^2}{h^2\Nzc^2} \notag \\
		&= 3\cdot(8\pi)^2\cdot \omega^2\cdot \frac{\SD{\obs}^2}{g(\Nzc)\Nzc^2}.
\end{align}

Rewriting in terms of total time: $t_n = (n\cdot\pi - \phi)/\omega$, $T_{tot} = (\Nzc\cdot\pi-\phi)/\omega$, and
\begin{equation}
	\SE{\hat{\omega}} = 8\pi^2\sqrt{3}\cdot\frac{\SD{\obs}}{\sqrt{\tilde{g}(T_{tot})}\cdot\bkt{T_{tot} + \phi/\omega}}, ~ \tilde{g}(T_{tot}) = \frac{1-\exp{\bkt{-\frac{T_{tot}}{\tau_d} - \frac{\phi/\omega}{\tau_d}}}}{1-\exp{(-\sfrac{\pi}{\omega\tau_d})}}.
\end{equation}

	
\paragraph{Simplifying.}
Let $\phi = 0$, then
\[
	\SE{\hat{\omega}} = 8\pi^2\sqrt{3}\cdot\sqrt{\frac{\bkt{1-e^{-\sfrac{\pi}{\omega\tau_d}}}}{\bkt{1 - e^{-T_{tot}/\tau_d}}}}\cdot\frac{\SD{\obs}}{T_{tot}}.
\]

If there's no spin tune decoherence, $\lambda = -1/\tau_d = 0$ and
\[
	\SE{\hat{\omega}} = 8\pi^2\sqrt{3}\cdot \sqrt{\frac{\pi}{\omega T_{tot}}}\cdot\frac{\SD{\obs}}{ T_{tot}}.
\]

The $\sqrt{\sfrac{\pi}{\omega T_{tot}}}$ factor just means that to get enough nodes from a slow signal one must measure it longer.

\end{document}

